Fix MerkleTree.EverCrypt.fst

secure_api/merkle_tree/MerkleTree.EverCrypt.fst
@@ -9,6 +9,7 @@ module HST = FStar.HyperStack.ST
 module MTH = MerkleTree.New.High
 module MTLD = MerkleTree.Low.Datastructures
 module MLH = MerkleTree.Low.Hashfunctions
+module Hash = Spec.Hash.Definitions
 
 open LowStar.Regional
 
@@ -42,16 +43,18 @@ let mt_sha256_compress src1 src2 dst =
                     (Rgl?.r_repr(hreg hash_size) hh0 src2))
                   (B.as_seq hh1 cb));
 
-  EHS.update #(Ghost.hide hash_alg) st cb;
+  EHS.update #(Ghost.hide hash_alg) st 0UL cb;
   let hh2 = HST.get () in
-  assert (EHS.repr st hh2 == Spec.Agile.Hash.update hash_alg (Spec.Agile.Hash.init hash_alg) (B.as_seq hh1 cb));
+  assert ((EHS.repr st hh2, ()) ==
+            Spec.Agile.Hash.update hash_alg (Spec.Agile.Hash.init hash_alg)
+                                            (B.as_seq hh1 cb));
   assert (S.equal (S.append S.empty (B.as_seq hh1 cb))
                   (B.as_seq hh1 cb));
 
   EHS.finish #(Ghost.hide hash_alg) st dst;
   let hh3 = HST.get () in
   assert (S.equal (B.as_seq hh3 dst)
-                  (Spec.Hash.PadFinish.finish hash_alg (EHS.repr st hh2)));
+                  (Spec.Hash.PadFinish.finish hash_alg (EHS.repr st hh2, ())));
   assert (S.equal (B.as_seq hh3 dst)
                   (Spec.Hash.PadFinish.finish hash_alg (Spec.Agile.Hash.update hash_alg (Spec.Agile.Hash.init hash_alg) (B.as_seq hh1 cb))));
   assert (S.equal (B.as_seq hh3 dst)
